src/Lean/Server/FileWorker.lean
@@ -402,7 +402,7 @@ def setupImports
     let progressDiagnostic := {
       range      := ⟨⟨0, 0⟩, ⟨1, 0⟩⟩
       -- make progress visible anywhere in the file
-      fullRange? := some ⟨⟨0, 0⟩, doc.text.utf8PosToLspPos doc.text.source.endPos⟩
+      fullRange? := some ⟨⟨0, 0⟩, doc.text.utf8PosToLspPos doc.text.source.rawEndPos⟩
       severity?  := DiagnosticSeverity.information
       message    := stderrLine
     }
